backend/Lineartyping.v
@@ -472,14 +472,7 @@ Proof.
 Qed.
 
 (* relies on x86-specific proofs *)
-Theorem wt_entry_point:
-  forall m S fp args, entry_point prog m S fp args -> wt_state S.
-Proof.
-  induction 1. econstructor.
-  constructor. constructor. apply Genv.find_funct_ptr_inversion in H4 as [id IN%wt_prog]; auto. reflexivity. apply wt_build_from_arguments; auto.
-  unfold ge0 in H2. apply Genv.find_funct_ptr_inversion in H2 as [id IN]. eapply wt_prog; eauto.
-  apply wt_build_from_arguments; auto.
-Admitted.
+
 
 End SOUNDNESS.
 
